code/ecdsap256/Hacl.Impl.ECDSA.MM.Exponent.fst
@@ -172,10 +172,10 @@ let montgomery_ladder_exponent #c r =
   pop_frame()  
 
 
-let fromDomainImpl a result = 
+let fromDomainImpl #c a result = 
   push_frame();
     let one = create (size 4) (u64 0) in 
-    uploadOneImpl one;
+    uploadOneImpl #c one;
     montgomery_multiplication_ecdsa_module one a result;
   pop_frame()   
 
