code/ecdsap256/Hacl.Impl.P256.MM.Exponent.fsti
@@ -7,34 +7,15 @@ module ST = FStar.HyperStack.ST
 open Lib.IntTypes
 open Lib.Buffer
 
-open FStar.Math.Lemmas
-open Hacl.Impl.P256.Math 
-
-open Hacl.Impl.P256.LowLevel 
-open FStar.Tactics
-open FStar.Tactics.Canon 
-
-open FStar.Mul
-
-open Lib.Loops
-
-open Hacl.Impl.P256.MontgomeryMultiplication
 open Hacl.Spec.P256.MontgomeryMultiplication
-
-open Hacl.Impl.P256.LowLevel.PrimeSpecific
-open Hacl.Impl.P256.Core
-open Hacl.Impl.P256.Arithmetics
-
 open Hacl.Spec.P256.Definition
-(* open Spec.P256.Lemmas *)
 open Spec.P256
-open Hacl.Spec.P256.MontgomeryMultiplication
 
-inline_for_extraction noextract
+
 val square_root: #c: curve -> a: felem c -> result: felem c -> Stack unit 
   (requires fun h -> live h a /\ live h result /\ as_nat c h a < prime256)
   (ensures fun h0 _ h1 -> modifies (loc a |+| loc result) h0 h1 /\
     as_nat c h1 result < prime256 /\
-    fromDomain_ #c (as_nat c h1 result) = sq_root_spec (fromDomain_ #c (as_nat c h0 a)) /\
-    fromDomain_ #c (as_nat c h1 result) = pow (fromDomain_ #c (as_nat c h0 a)) ((prime256 + 1) / 4) % prime256
+    fromDomain_ #c (as_nat c h1 result) = sq_root_spec #c (fromDomain_ #c (as_nat c h0 a)) /\
+    fromDomain_ #c (as_nat c h1 result) = pow (fromDomain_ #c (as_nat c h0 a)) ((getPrime c+ 1) / 4) % getPrime c
   )
