code/ecdsap256/Hacl.Impl.SolinasReduction.fst
@@ -151,9 +151,10 @@ let upl_zer_buffer c0 c1 c2 c3 c4 c5 c6 c7 o =
     assert(v b3 = v c7 * pow2 32 + v c6);
 
     load_buffer b0 b1 b2 b3 o;
-    reduction_prime_2prime_impl o o;
+    reduction_prime_2prime #P256 o o;
     let h2 = ST.get() in
     assert(as_nat P256 h2 o = (v c1 * pow2 32 + v c0 + v c3 * pow2 (3 * 32) + v c2 * pow2 (2 * 32) + v c5 * pow2 (32 * 5) + v c4 * pow2 (32 * 4) + v c7 * pow2 (32 * 7) + v c6 * pow2 (32 * 6)) % prime256)
+
 
 inline_for_extraction noextract
 val upl_fir_buffer: c11: uint32 -> c12: uint32 -> c13: uint32 -> c14: uint32 -> c15: uint32
@@ -176,7 +177,7 @@ let upl_fir_buffer c11 c12 c13 c14 c15 o =
   let b2 = store_high_low_u c13 c12 in
   let b3 = store_high_low_u c15 c14 in
   load_buffer b0 b1 b2 b3 o;
-  reduction_prime_2prime_impl o o
+  reduction_prime_2prime #P256 o o
 
 inline_for_extraction noextract
 val upl_sec_buffer: c12: uint32 -> c13: uint32 -> c14: uint32 -> c15: uint32
@@ -222,7 +223,7 @@ let upl_thi_buffer c8 c9 c10 c14 c15 o =
    let b2 = u64 0 in
    let b3 = store_high_low_u c15 c14 in
    load_buffer b0 b1 b2 b3 o;
-   reduction_prime_2prime_impl o o
+   reduction_prime_2prime #P256 o o
 
 inline_for_extraction noextract
 val upl_for_buffer: c8: uint32 -> c9: uint32 -> c10: uint32 -> c11: uint32 -> c13: uint32 ->
@@ -243,7 +244,7 @@ let upl_for_buffer c8 c9 c10 c11 c13 c14 c15 o =
   let b2 = store_high_low_u c15 c14 in
   let b3 = store_high_low_u c8 c13 in
   load_buffer b0 b1 b2 b3 o;
-  reduction_prime_2prime_impl o o
+  reduction_prime_2prime #P256 o o
 
 inline_for_extraction noextract
 val upl_fif_buffer: c8: uint32 -> c10: uint32 -> c11: uint32 -> c12: uint32 -> c13: uint32
@@ -264,7 +265,7 @@ let upl_fif_buffer c8 c10 c11 c12 c13 o =
     let b2 = u64 0 in
     let b3 = store_high_low_u c10 c8 in
     load_buffer b0 b1 b2 b3 o;
-    reduction_prime_2prime_impl o o
+    reduction_prime_2prime #P256 o o
 
 inline_for_extraction noextract
 val upl_six_buffer: c9: uint32 -> c11: uint32 -> c12: uint32 -> c13: uint32 -> c14: uint32 -> c15: uint32-> 
@@ -286,7 +287,7 @@ let upl_six_buffer c9 c11 c12 c13 c14 c15 o =
     let b2 = u64 0 in
     let b3 = store_high_low_u c11 c9 in
     load_buffer b0 b1 b2 b3 o;
-    reduction_prime_2prime_impl o o
+    reduction_prime_2prime #P256 o o
 
 inline_for_extraction noextract
 val upl_sev_buffer: c8: uint32 -> c9: uint32 -> c10: uint32 -> c12: uint32 -> c13: uint32 ->
@@ -308,7 +309,7 @@ let upl_sev_buffer c8 c9 c10 c12 c13 c14 c15 o =
     let b2 = store_high_low_u c10 c9 in
     let b3 = store_high_low_u c12 (u32 0) in
     load_buffer b0 b1 b2 b3 o;
-    reduction_prime_2prime_impl o o
+    reduction_prime_2prime #P256 o o
 
 inline_for_extraction noextract
 val upl_eig_buffer: c9: uint32 -> c10: uint32 -> c11: uint32 -> c12: uint32 -> c13: uint32 ->
@@ -329,7 +330,7 @@ let upl_eig_buffer c9 c10 c11 c12 c13 c14 c15 o =
     let b2 = store_high_low_u c11 c10 in
     let b3 = store_high_low_u c13 (u32 0) in
     load_buffer b0 b1 b2 b3 o;
-    reduction_prime_2prime_impl o o
+    reduction_prime_2prime #P256 o o
 
 
 inline_for_extraction noextract
@@ -426,16 +427,16 @@ let solinas_reduction_operations tempBuffer o =
     let t7 = sub tempBuffer (size 28) (size 4) in
     let t8 = sub tempBuffer (size 32) (size 4) in
 
-    p256_double t2 t2;
-    p256_double t1 t1;
-    p256_add t0 t1 o;
-    p256_add t2 o o;
-    p256_add t3 o o;
-    p256_add t4 o o;
-    p256_sub o t5 o;
-    p256_sub o t6 o;
-    p256_sub o t7 o;
-    p256_sub o t8 o;
+    felem_double #P256 t2 t2;
+    felem_double #P256 t1 t1;
+    felem_add #P256 t0 t1 o;
+    felem_add #P256 t2 o o;
+    felem_add #P256 t3 o o;
+    felem_add #P256 t4 o o;
+    felem_sub #P256 o t5 o;
+    felem_sub #P256 o t6 o;
+    felem_sub #P256 o t7 o;
+    felem_sub #P256 o t8 o;
 
     reduce_brackets (as_nat P256 h0 t0) (as_nat P256 h0 t1) (as_nat P256 h0 t2) (as_nat P256 h0 t3) (as_nat P256 h0 t4) (as_nat P256 h0 t5) (as_nat P256 h0 t6) (as_nat P256 h0 t7) (as_nat P256 h0 t8)
 
